Accidentally replaced CoreCrypto from outsourced signature branch... restoring

ucontrib/CoreCrypto/fst/CoreCrypto.fst
@@ -31,6 +31,8 @@ assume val digest_final : hash_ctx -> EXT bytes
 
 (* --------------------------- *)
 
+
+type sig_alg = | RSASIG | DSA | ECDSA | RSAPSS
 type block_cipher = | AES_128_CBC | AES_256_CBC | TDES_EDE_CBC
 type stream_cipher = | RC4_128
 type rsa_padding = | Pad_none | Pad_PKCS1
@@ -200,3 +202,31 @@ type ec_key = {
 
 assume val ec_is_on_curve: ec_params -> ec_point -> Tot bool
 assume val ecdh_agreement: k:ec_key{Some? k.ec_priv} -> ec_point -> EXT bytes
+
+assume val ecdsa_sign: option hash_alg -> k:ec_key{Some? k.ec_priv} -> bytes -> EXT bytes
+assume val ecdsa_verify: option hash_alg -> ec_key -> bytes -> bytes -> EXT bool
+assume val ec_gen_key: p:ec_params
+  -> EXT (k:ec_key{Some? k.ec_priv /\ k.ec_params = p /\
+                  length k.ec_point.ecx = ec_bytelen k.ec_params.curve /\
+                  length k.ec_point.ecy = ec_bytelen k.ec_params.curve})
+
+//TODO: keep also abtsract OpenSSL representation for efficiency?
+type key =
+  | KeyRSA of rsa_key
+  | KeyDSA of dsa_key
+  | KeyECDSA of ec_key
+
+// If we are careless we can cause openssl segfaults when signing or encrypting
+// with keys that are missing the "private" field.
+// The only has_priv keys are the ones loaded with load_key and or generated with gen_key
+let has_priv : key -> Type0 = function
+  | KeyRSA k -> Some? k.rsa_prv_exp
+  | KeyDSA k -> Some? k.dsa_private
+  | KeyECDSA k -> Some? k.ec_priv
+
+assume val validate_chain: der_list:list bytes -> for_signing:bool -> hostname:option string -> ca_file:string -> Tot bool
+assume val get_key_from_cert: bytes -> Tot (option key)
+assume val hash_and_sign: k:key{has_priv k} -> hash_alg -> bytes -> Tot bytes
+assume val verify_signature: key -> hash_alg -> tbs:bytes -> sigv:bytes -> Tot bool
+assume val load_chain: pemfile:string -> Tot (option (list bytes))
+assume val load_key: keyfile:string -> Tot (option (k:key{has_priv k}))
